progress on compiler correctness
change to intermediate language semantics: require closure values to
store their environtment alists in sorted order, and all distinct, so
that they are canonical. use the fact that the types are countable to
generate the order by which they are sorted.

examples/miniML/compiler/compileCorrectnessScript.sml
@@ -1,4 +1,4 @@
-open HolKernel bossLib boolLib MiniMLTheory evaluateEquationsTheory compileTerminationTheory listTheory lcsymtacs
+open HolKernel bossLib boolLib MiniMLTheory evaluateEquationsTheory compileTerminationTheory count_expTheory listTheory lcsymtacs
 
 val _ = new_theory "compileCorrectness"
 
@@ -88,6 +88,14 @@ val well_typed_App_subexp = store_thm(
 rw[] >> match_mp_tac (MP_CANON well_typed_subexp_lem) >>
 metis_tac [subexp_rules])
 
+(* TODO: move? *)
+
+val lookup_ALOOKUP = store_thm(
+"lookup_ALOOKUP",
+``lookup = combin$C ALOOKUP``,
+fs[FUN_EQ_THM] >> gen_tac >> Induct >- rw[] >> Cases >> rw[])
+val _ = export_rewrites["lookup_ALOOKUP"];
+
 (* nicer induction theorem for evaluate *)
 (* TODO: move? *)
 
@@ -153,10 +161,12 @@ evaluate_ind
 
 (* TODO: save in compileTerminationTheory? *)
 val Cevaluate_cases = CompileTheory.Cevaluate_cases
+val Cevaluate_rules = CompileTheory.Cevaluate_rules
 val extend_def = CompileTheory.extend_def
 val exp_Cexp_ind = CompileTheory.exp_Cexp_ind
 val v_Cv_ind = CompileTheory.v_Cv_ind
 val v_Cv_cases = CompileTheory.v_Cv_cases
+val sort_Cenv_def = CompileTheory.sort_Cenv_def
 
 (* Cevaluate functional equations *)
 
@@ -170,7 +180,72 @@ val Cevaluate_val = store_thm(
 ``∀env v res. Cevaluate env (CVal v) res = (res = Rval v)``,
 rw[Once Cevaluate_cases])
 
-val _ = export_rewrites["Cevaluate_raise","Cevaluate_val"]
+val Cevaluate_var = store_thm(
+"Cevaluate_var",
+``∀env vn res. Cevaluate env (CVar vn) res = (res = Rval (env ' vn))``,
+rw[Once Cevaluate_cases])
+
+val _ = export_rewrites["Cevaluate_raise","Cevaluate_val","Cevaluate_var"]
+
+val Cevaluate_con = store_thm(
+"Cevaluate_con",
+``∀env cn es res. Cevaluate env (CCon cn es) res =
+(∃vs. Cevaluate_list env es (Rval vs) ∧ (res = Rval (CConv cn vs))) ∨
+(∃err. Cevaluate_list env es (Rerr err) ∧ (res = Rerr err))``,
+rw[Once Cevaluate_cases] >> PROVE_TAC[])
+
+val (Cevaluate_list_with_rules,Cevaluate_list_with_ind,Cevaluate_list_with_cases) = Hol_reln [ANTIQUOTE(
+Cevaluate_rules |> SIMP_RULE (srw_ss()) [] |> concl |>
+strip_conj |>
+Lib.filter (fn tm => tm |> strip_forall |> snd |> strip_imp |> snd |> strip_comb |> fst |> same_const ``Cevaluate_list``) |>
+let val t1 = ``Cevaluate env``
+    val t2 = ``Cevaluate_list env``
+    val tP = type_of t1
+    val P = mk_var ("P",tP)
+    val ew = mk_comb(mk_var("Cevaluate_list_with",tP --> type_of t2),P)
+in List.map (fn tm => tm |> strip_forall |> snd |>
+                   subst [t1|->P, t2|->ew])
+end |> list_mk_conj)]
+
+val Cevaluate_list_with_Cevaluate = store_thm(
+"Cevaluate_list_with_Cevaluate",
+``∀env. Cevaluate_list env = Cevaluate_list_with (Cevaluate env)``,
+gen_tac >>
+simp_tac std_ss [Once FUN_EQ_THM] >>
+Induct >>
+rw[FUN_EQ_THM] >-
+  rw[Once Cevaluate_cases,Once Cevaluate_list_with_cases] >>
+rw[Once Cevaluate_cases] >>
+rw[Once Cevaluate_list_with_cases,SimpRHS] >>
+PROVE_TAC[])
+
+val evaluate_list_with_nil = store_thm(
+"evaluate_list_with_nil",
+``∀f res. evaluate_list_with f [] res = (res = Rval [])``,
+rw[Once evaluate_list_with_cases])
+val _ = export_rewrites["evaluate_list_with_nil"];
+
+val evaluate_list_with_cons = store_thm(
+"evaluate_list_with_cons",
+``∀f e es res. evaluate_list_with f (e::es) res =
+  (∃v vs. f e (Rval v) ∧ evaluate_list_with f es (Rval vs) ∧ (res = Rval (v::vs))) ∨
+  (∃v err. f e (Rval v) ∧ evaluate_list_with f es (Rerr err) ∧ (res = Rerr err)) ∨
+  (∃err. f e (Rerr err) ∧ (res = Rerr err))``,
+rw[Once evaluate_list_with_cases] >> PROVE_TAC[])
+
+val Cevaluate_list_with_nil = store_thm(
+"Cevaluate_list_with_nil",
+``∀f res. Cevaluate_list_with f [] res = (res = Rval [])``,
+rw[Once Cevaluate_list_with_cases])
+val _ = export_rewrites["Cevaluate_list_with_nil"];
+
+val Cevaluate_list_with_cons = store_thm(
+"Cevaluate_list_with_cons",
+``∀f e es res. Cevaluate_list_with f (e::es) res =
+  (∃v vs. f e (Rval v) ∧ Cevaluate_list_with f es (Rval vs) ∧ (res = Rval (v::vs))) ∨
+  (∃v err. f e (Rval v) ∧ Cevaluate_list_with f es (Rerr err) ∧ (res = Rerr err)) ∨
+  (∃err. f e (Rerr err) ∧ (res = Rerr err))``,
+rw[Once Cevaluate_list_with_cases] >> PROVE_TAC[])
 
 val good_cm_cw_def = Define`
   good_cm_cw cm cw =
@@ -283,6 +358,126 @@ qsuff_tac `∀b cm s exp s' Cexp.
   (FST (s,exp)).m SUBMAP s'.m` >- rw[] >>
 ho_match_mp_tac exp_to_Cexp_ind >>
 rw[exp_to_Cexp_def,extend_def]
+*)
+
+val good_cmap_def = Define`
+good_cmap cenv cm =
+  (∀cn n. do_con_check cenv cn n ⇒ cn IN FDOM cm)`
+
+val good_exp_to_Cexp_state_def = Define`
+  good_exp_to_Cexp_state env s =
+  INJ (FAPPLY s.m) (set (MAP FST env)) UNIV`
+
+(* TODO: move? *)
+val QSORT_eq_if_PERM = store_thm(
+"QSORT_eq_if_PERM",
+``!R l1 l2. total R /\ transitive R /\ antisymmetric R /\ PERM l1 l2 ==> (QSORT R l1 = QSORT R l2)``,
+PROVE_TAC[sortingTheory.QSORT_PERM,sortingTheory.QSORT_SORTED,sortingTheory.SORTED_PERM_EQ,
+          sortingTheory.PERM_TRANS,sortingTheory.PERM_SYM])
+
+local open pred_setTheory relationTheory in
+(* TODO: move, or use set_relation stuff? *)
+val countable_has_linear_order = store_thm(
+"countable_has_linear_order",
+``countable (UNIV:'a set) ==>
+  ?(r:'a->'a->bool). antisymmetric r /\ transitive r /\ total r``,
+SRW_TAC[][countable_def,INJ_DEF] THEN
+Q.EXISTS_TAC `inv_image $<= f` THEN
+SRW_TAC[][antisymmetric_def,
+          transitive_def,
+          total_def,
+          inv_image_def] THEN
+METIS_TAC[arithmeticTheory.LESS_EQUAL_ANTISYM,
+          arithmeticTheory.LESS_EQ_TRANS,
+          arithmeticTheory.LESS_EQ_CASES])
+end
+
+(*
+val exp_to_Cexp_thm1 = store_thm(
+"exp_to_Cexp_thm1",
+``∀tp cm Ps Pexp s exp s' Cexp cenv env res.
+  ((Ps,Pexp) = (s,exp)) ∧
+  good_exp_to_Cexp_state env s ∧
+  (exp_to_Cexp tp cm (s,exp) = (s',Cexp)) ∧
+  (tp = F) ∧
+  evaluate cenv env exp res ∧
+  (res ≠ Rerr Rtype_error) ∧
+  good_cmap cenv cm ⇒
+  Cevaluate (alist_to_fmap (MAP (λ(x,v). (s.m ' x, v_to_Cv cm (s,v))) env)) Cexp (map_result (λv. v_to_Cv cm (s,v)) res)``,
+ho_match_mp_tac exp_to_Cexp_ind >>
+strip_tac >-
+  fs[exp_to_Cexp_def] >>
+strip_tac >-
+  fs[exp_to_Cexp_def,v_to_Cv_def] >>
+strip_tac >- (
+  fs[exp_to_Cexp_def] >>
+  rw[Cevaluate_con,evaluate_con] >>
+  fs[Cevaluate_list_with_Cevaluate,evaluate_list_with_evaluate] >>
+  qpat_assum `do_con_check cenv cn (LENGTH es)` kall_tac >>
+  rw[] >>
+  TRY (qpat_assum `X Y Z (Rval vs)` mp_tac >> qid_spec_tac `vs`) >>
+  Induct_on `es` >- (
+    rw[Once evaluate_cases, Once Cevaluate_cases] ) >>
+  fs[v_to_Cv_def] >- (
+    rw[] >>
+    fs[evaluate_list_with_cons] >- (
+      rw[Cevaluate_list_with_cons] >>
+      disj1_tac >>
+      qmatch_assum_abbrev_tac `P ⇒ Q ⇒ R` >>
+      `R` by metis_tac[] >>
+      qpat_assum `Q` kall_tac >>
+      qpat_assum `P ⇒ Q ⇒ R` kall_tac >>
+      unabbrev_all_tac >>
+      first_x_assum (qspec_then `h` mp_tac) >> rw[] >>
+      first_x_assum (qspecl_then [`cenv`,`env`,`Rval v`] mp_tac) >> rw[] >>
+      metis_tac[] ) >>
+    rw[Cevaluate_list_with_cons] >>
+    disj2_tac >>
+    first_x_assum (qspec_then `h` mp_tac) >> rw[] >>
+    first_x_assum (qspecl_then [`cenv`,`env`,`Rerr err`] mp_tac) >> rw[] ) >>
+  rw[] >>
+  fs[evaluate_list_with_cons] >>
+  rw[Cevaluate_list_with_cons] >- (
+    first_x_assum (qspec_then `h` mp_tac) >> rw[] >>
+    first_x_assum (qspecl_then [`cenv`,`env`,`Rval v`] mp_tac) >> rw[] ) >>
+  first_x_assum (match_mp_tac o MP_CANON) >>
+  rw[] >>
+  metis_tac[] ) >>
+strip_tac >- (
+  fs[exp_to_Cexp_def,evaluate_var] >>
+  rw[] >> rw[] >>
+  fs[good_exp_to_Cexp_state_def] >>
+  qho_match_abbrev_tac `x = alist_to_fmap (MAP (λ(x,y). (f1 x, f2 y)) al) ' z` >>
+  `f1 = FAPPLY s.m` by rw[Abbr`f1`,FUN_EQ_THM] >>
+  rw[alistTheory.alist_to_fmap_MAP] >>
+  `vn IN FDOM (f2 o_f alist_to_fmap al)` by (
+    rw[MEM_MAP] >>
+    imp_res_tac alistTheory.ALOOKUP_MEM >>
+    qexists_tac `(vn,v)` >> rw[] ) >>
+  rw[finite_mapTheory.MAP_KEYS_def,Abbr`z`] >>
+  unabbrev_all_tac >>
+  rw[finite_mapTheory.o_f_DEF] >>
+  imp_res_tac alistTheory.ALOOKUP_SOME_FAPPLY_alist_to_fmap >>
+  rw[] ) >>
+strip_tac >- (
+  fs[exp_to_Cexp_def] >>
+  rw[v_to_Cv_def] >>
+  fs[LET_THM] >>
+  rw[Once Cevaluate_cases] >>
+  rw[sort_Cenv_def] >>
+  match_mp_tac QSORT_eq_if_PERM >>
+  simp_tac(srw_ss())[CONJ_ASSOC] >>
+  conj_tac >- (
+    fs[fsetTheory.a_linear_order_def] >>
+    SELECT_ELIM_TAC >> rw[] >>
+    match_mp_tac countable_has_linear_order >>
+    rw[pred_setTheory.countable_def] >>
+    qexists_tac `count_prod_aux count_num_aux count_Cv_aux` >>
+    rw[pred_setTheory.INJ_DEF] ) >>
+  rw[Once sortingTheory.PERM_SYM] >>
+  match_mp_tac alistTheory.alist_to_fmap_to_alist_PERM >>
+  rw[Abbr`Cenv`,MAP_MAP_o]
+  good_exp_to_Cexp_state_def
 *)
 
 (*
